change length/nth to Zlength/Znth

heap/list_relation.v
@@ -1,6 +1,10 @@
 Require Import FloydSeq.proofauto.
-(* Require Import cprogs.heap.program. *)
+(* Require Import cprogs.heap_list_down.program. *)
 Require Import Notations Logic Datatypes.
+Require Export Coq.Classes.Init.
+(* Require Import Coq.Program.Basics. *)
+Require Import Coq.Program.Tactics.
+Require Import Coq.Relations.Relation_Definitions.
 From Coq Require Import String List ZArith. 
 From compcert Require Import Coqlib Integers Floats AST Ctypes Cop Clight Clightdefs.
 
@@ -13,60 +17,129 @@ Local Open Scope list_scope.
 Require Import SetsClass.SetsClass.
 Local Open Scope sets.
 Import SetsNotation.
+Lemma list_equal : forall (A: Type) (l1 l2: list A) {d: Inhabitant A},
+  l1 = l2 <-> Zlength l1 = Zlength l2 /\
+  forall (i: Z), 0 <= i < Zlength l1 -> Znth i l1 = Znth i l2.
+Proof.
+  split.
+  + intros.
+    rewrite H.
+    tauto.
+  + intros.
+    destruct H.
+    apply (Znth_eq_ext l1 l2); [tauto | tauto].
+Qed.
 
-Definition list_swap (x: nat) (y: nat):
+Definition list_swap (x: Z) (y: Z):
   list Z -> list Z -> Prop :=
   fun l1 l2 =>
-    length l1 = length l2 /\
-    nth x l1 0 = nth y l2 0 /\ nth y l1 0 = nth x l2 0 /\
-    forall i, (i < length l1)%nat /\ i <> x /\ i <> y ->
-      nth i l1 0 = nth i l2 0.
+    Zlength l1 = Zlength l2 /\
+    Znth x l1 = Znth y l2 /\ Znth y l1 = Znth x l2 /\
+    forall i, 0 <= i < Zlength l1 /\ i <> x /\ i <> y ->
+      Znth i l1 = Znth i l2.
 
 Import ListNotations.
 
 Require Import BinNums.
 Require Coq.micromega.Lia.
 
-Definition state: Type := ((list Z) * nat).
+Definition list_state: Type := ((list Z) * Z).
 
-Definition get_num(l: state): Z := 
-  nth ((snd l) - 1) (fst l) 0.
+Definition get_list_val(l: list_state): Z := 
+  Znth ((snd l)) (fst l).
+
+Definition legal_list_state(l: list_state): Prop:=
+  ((snd l) <= Zlength (fst l)) /\ 1 <= (snd l).
 
 Definition list_up_succeed:
-  state -> state -> Prop :=
-  fun l1 l2 =>
-    (1%nat < (snd l1))%nat /\ ((snd l2) = (snd l1)/2)%nat /\
-    get_num l1 > (nth ((snd l2)-1) (fst l1) 0) /\
-    (list_swap ((snd l1)-1) ((snd l2)-1) (fst l1) (fst l2)).
+  list_state -> list_state -> Prop :=
+  fun l1 l2 => legal_list_state l1 /\ legal_list_state l2 /\
+    1 < (snd l1) /\ (snd l2) = (snd l1) / 2 /\
+    get_list_val l1 > (Znth (snd l2) (fst l1)) /\
+    (list_swap (snd l1) (snd l2) (fst l1) (fst l2)).
 
 Definition list_up_fail:
-  state -> state -> Prop:=
-  Rels.test(fun l =>
-    (1%nat = (snd l))%nat \/
-    ((1%nat < (snd l))%nat /\ 
-    get_num l <= (nth ((snd l)/2) (fst l) 0))).
+  list_state -> list_state -> Prop:=
+  Rels.test(fun l =>  legal_list_state l /\
+    (1 = (snd l) \/
+    (1 < (snd l) /\ 
+    get_list_val l <= (Znth ((snd l) / 2) (fst l))))).
 
-Fixpoint iter_n (n: nat):
-  state -> state -> Prop :=
+Fixpoint iter_n_list_up (n: nat):
+  list_state -> list_state -> Prop :=
   match n with
   | O => list_up_fail
-  | S n0 => list_up_succeed ∘ (iter_n n0)
+  | S n0 => list_up_succeed ∘ (iter_n_list_up n0)
   end.
 
-Definition heap_up:
-  state -> state -> Prop :=
-  ⋃ (iter_n).
+Definition heap_list_up:
+  list_state -> list_state -> Prop :=
+  ⋃ (iter_n_list_up).
 
-Example test : list_swap 2%nat 1%nat [2; 3; 4; 5] [2; 4; 3; 5].
+Definition left_son(l: list_state): list_state :=
+  pair (fst l) ((snd l) * 2).
+
+Definition left_son_swap(l1 l2: list_state): Prop :=
+  (list_swap (snd l1) (snd l2) (fst l1) (fst l2)) /\ (snd l1) * 2 = (snd l2).
+  
+Definition right_son_swap(l1 l2: list_state): Prop :=
+  (list_swap (snd l1) (snd l2) (fst l1) (fst l2)) /\ (snd l1) * 2 + 1 = (snd l2).
+
+Definition right_son(l: list_state): list_state :=
+  pair (fst l) ((snd l) * 2 + 1).
+
+Definition left_son_check_list (l: list_state): Prop :=
+  legal_list_state (left_son l) /\
+  get_list_val l < get_list_val (left_son l).
+  
+Definition right_son_check_list (l: list_state): Prop :=
+  legal_list_state (right_son l) /\
+  get_list_val l < get_list_val (right_son l).
+
+Definition list_down_succeed:
+  list_state -> list_state -> Prop :=
+  fun l1 l2 =>
+    ((left_son_check_list l1) /\ ~(right_son_check_list l1) /\ (left_son_swap l1 l2)) \/
+    ((left_son_check_list l1) /\ (right_son_check_list l1) /\ (
+      ((get_list_val (left_son l1)) > (get_list_val (right_son l1)) /\ (left_son_swap l1 l2))  \/
+      ((get_list_val (left_son l1)) <= (get_list_val (right_son l1)) /\ (right_son_swap l1 l2))
+    )) \/
+    (~(left_son_check_list l1) /\ (right_son_check_list l1) /\ (right_son_swap l1 l2)).
+
+Definition list_down_fail:
+  list_state -> list_state -> Prop :=
+  Rels.test(fun l =>
+    ~(left_son_check_list l) /\ ~(right_son_check_list l)).
+
+Fixpoint iter_n_list_down (n: nat):
+  list_state -> list_state -> Prop :=
+  match n with
+  | O => list_down_fail
+  | S n0 => list_down_succeed ∘ (iter_n_list_down n0)
+  end.
+
+Definition heap_list_down:
+  list_state -> list_state -> Prop :=
+  ⋃ (iter_n_list_down).
+
+Ltac simpl_Z :=
+  simpl; unfold Zlength, Zlength_aux; unfold Znth; simpl.
+
+Ltac try_list_unfold :=
+  unfold left_son_check_list; unfold left_son_swap; unfold left_son; 
+  unfold right_son_check_list; unfold right_son_swap; unfold right_son;
+  unfold get_list_val; unfold legal_list_state; simpl_Z.
+
+Example test : list_swap 2 1 [2; 3; 4; 5] [2; 4; 3; 5].
 Proof.
   unfold list_swap.
-  unfold length.
-  unfold nth at 1 2 3 4.
+  unfold Zlength, Zlength_aux.
+  unfold Znth at 1 2 3 4.
   split; [tauto | ].
   split; [tauto | ].
   split; [tauto | ].
   intros.
-  assert (i = 0%nat \/ i = 3%nat) by lia.
+  assert (i = 0 \/ i = 3) by lia.
   destruct H0.
   + rewrite H0.
     tauto.
@@ -74,101 +147,111 @@ Proof.
     tauto.  
 Qed.
 
-Example check_succeed : list_up_succeed (pair [2; 3; 4; 5] 2%nat) (pair [3; 2; 4; 5] 1%nat).
+Example check_succeed_up : list_up_succeed (pair [233;2; 3; 4; 5] 2) (pair [233;3; 2; 4; 5] 1).
 Proof.
   unfold list_up_succeed.
+  split; [unfold legal_list_state; simpl_Z; lia|].
+  split; [unfold legal_list_state; simpl_Z; lia|].
   split; [simpl; lia|].
   split; [simpl; tauto|].
-  split; [unfold get_num; simpl; lia|].
+  split; [unfold get_list_val; simpl_Z; lia|].
   simpl.
-  unfold list_swap. unfold length.
+  unfold list_swap. simpl_Z.
   split; [tauto|].
   split; [tauto|].
   split; [tauto|].
   intros.
   destruct H as [H0 [H1 H2]].
-  assert (i = 2%nat \/ i = 3%nat) by lia.
+  assert (i = 0 \/ i = 3 \/ i = 4) by lia.
+  destruct H;[ subst; tauto|].
   destruct H; subst; tauto.
 Qed.
 
-Example check_heap_up : heap_up (pair [2; 3; 4; 5] 2%nat) (pair [3; 2; 4; 5] 1%nat).
+Example check_heap_list_up : heap_list_up (pair [233;2; 3; 4; 5] 2) (pair [233;3; 2; 4; 5] 1).
 Proof.
-  unfold heap_up.
-  sets_unfold.
+  unfold heap_list_up.
+  unfold_RELS_tac.
   exists 1%nat.
-  unfold iter_n.
-  sets_unfold.
-  exists (pair [3; 2; 4; 5] 1%nat).
+  unfold iter_n_list_up.
+  unfold_RELS_tac.
+  exists (pair [233;3; 2; 4; 5] 1).
   split.
-  + apply check_succeed.
+  + apply check_succeed_up.
   + unfold list_up_fail.
     simpl.
     split.
-    - left; tauto.
-    - sets_unfold.
-      tauto.
+    - split; unfold legal_list_state; simpl_Z; lia.
+    - tauto.
 Qed.
 
-Example check_heap_up2 : heap_up (pair [100;3;2;5] 4%nat) (pair [100;5;2;3] 2%nat).
+Example check_heap_list_up2 : heap_list_up (pair [233;100;3;2;5] 4) (pair [233;100;5;2;3] 2).
 Proof.
-  unfold heap_up.
-  sets_unfold.
+  unfold heap_list_up.
+  unfold_RELS_tac.
   exists 1%nat.
-  unfold iter_n.
-  sets_unfold.
-  exists (pair [100;5;2;3] 2%nat).
+  unfold iter_n_list_up.
+  unfold_RELS_tac.
+  exists (pair [233;100;5;2;3] 2).
   split.
   + unfold list_up_succeed.
+    split; [unfold legal_list_state; simpl_Z; lia|].
+    split; [unfold legal_list_state; simpl_Z; lia|].
     split; [unfold snd; lia|].
     split; [unfold snd; tauto|].
-    split; [unfold get_num; simpl; lia|].
+    split; [unfold get_list_val; simpl_Z; lia|].
     simpl.
-    unfold list_swap. unfold length.
+    unfold list_swap. simpl_Z.
     split; [tauto|].
     split; [tauto|].
     split; [tauto|].
     intros.
     destruct H as [H0 [H1 H2]].
-    assert (i = 0%nat \/ i = 2%nat) by lia.
+    assert (i = 0 \/ i = 1 \/ i = 3) by lia.
+    destruct H;[ subst; tauto|].
     destruct H; subst; tauto.
   + unfold list_up_fail.
     simpl.
     split.
-    - right.
-      split; [lia|].
-      unfold get_num; simpl; lia.
-    - sets_unfold.
-      tauto.
+    - split.
+      unfold legal_list_state; simpl_Z; lia.
+      right; split; [lia|].
+      unfold get_list_val; simpl_Z; lia.
+    - tauto.
 Qed.
 
-Definition list_swap_rev (x: nat) (y: nat):
-  list Z -> list Z -> Prop := (list_swap x y) ∘ (list_swap x y).
-
-Lemma swap_rev: forall (x y: nat) (l1 l3: list Z),
-  (list_swap_rev x y) l1 l3 -> l1 = l3.
+Example check_succeed_down : list_down_succeed (pair [233;4;6;9;2;4;1;3] 1) (pair [233;9;6;4;2;4;1;3] 3).
 Proof.
-  intros ? ? ? ?.
-  unfold list_swap_rev.
-  sets_unfold.
-  (* unfold_RELS_tac. *)
-  unfold list_swap.
+  unfold list_down_succeed.
+  right; left.
+  split; try_list_unfold; [lia|].
+  split; [lia|].
+  right; split; [lia|].
+  unfold list_swap; simpl_Z.
+  split; [|tauto].
+  split; [tauto|].
+  split; [tauto|].
+  split; [tauto|].
   intros.
-  destruct H as [H [? ?] ].
-  destruct H0 as [? [? [? ?]]].
-  destruct H1 as [? [? [? ?]]].
-  rewrite <- H0 in H1, H7.
-  rewrite <- H3 in H5.
-  rewrite <- H2 in H6.
-  clear H0 H2 H3.
-  assert (forall (i: nat), (i < length l1)%nat -> nth i l1 0 = nth i l3 0). {
-    intros.
-    assert (i = x \/ i = y \/ (i < length l1)%nat /\ i <> x /\ i <> y) by lia.
-    destruct H2; [rewrite H2; tauto | ].
-    destruct H2; [rewrite H2; tauto | ].
-    specialize (H4 i H2).
-    specialize (H7 i H2).
-    rewrite H4.
-    apply H7.
-  }
-  apply (nth_ext l1 l3 0 0 H1 H0).
+  assert (i = 0 \/ i = 2 \/ i = 4 \/ i = 5 \/ i = 6 \/ i = 7) by lia.
+  destruct H0; [subst; tauto|].
+  destruct H0; [subst; tauto|].
+  destruct H0; [subst; tauto|].
+  destruct H0; [subst; tauto|].
+  destruct H0; subst; tauto.
 Qed.
+
+Example check_heap_list_down : heap_list_down (pair [233;4;6;9;2;4;1;3] 1) (pair [233;9;6;4;2;4;1;3] 3).
+Proof.
+  unfold heap_list_down.
+  unfold_RELS_tac.
+  exists 1%nat.
+  unfold iter_n_list_down.
+  unfold_RELS_tac.
+  exists ([233; 9; 6; 4; 2; 4; 1; 3], 3).
+  split.
+  + exact check_succeed_down.
+  + unfold list_down_fail.
+    simpl_Z; split; [|tauto].
+    try_list_unfold; lia.
+Qed.
+
