heap/tree_list.v
@@ -3,6 +3,7 @@ Require Import FloydSeq.proofauto.
 Require Import Notations Logic Datatypes.
 From Coq Require Import String List ZArith. 
 From compcert Require Import Coqlib Integers Floats AST Ctypes Cop Clight Clightdefs.
+Require Import Coq.Logic.Classical_Pred_Type.
 
 Require Import Coq.micromega.Psatz.
 Local Open Scope string.
@@ -80,4 +81,207 @@ Proof.
   apply list_to_tree3.
 Qed.
 
+Definition partial_tree: Type := list (bool * Z * tree).
+(* true:right_son is cut
+   false:left_son is cut*)
+Definition tree_state: Type := partial_tree * tree.
 
+Definition legal_tree_state (t: tree_state): Prop :=
+  exists v ls rs, (snd t) = Node v ls rs.
+
+Definition swap_up_and_combine (v: Z) (ls rs: tree) (t2: bool * Z * tree): tree :=
+  match (fst (fst t2)) with
+  | true => Node v (snd t2) (Node (snd (fst t2)) ls rs)  
+  | false => Node v (Node (snd (fst t2)) ls rs) (snd t2)
+  end.
+
+Definition get_tree_val (t: tree): Z :=
+  match (t) with
+  | Leaf => default
+  | Node v l r => v
+  end.
+
+Definition tree_up_succeed:
+  tree_state -> tree_state -> Prop:=
+    fun t1 t2 => exists t3 l', 
+    (t3::l' = (fst t1)) /\ (l' = (fst t2)) /\
+    (exists v ls rs, (swap_up_and_combine v ls rs t3) = (snd t2) /\ (snd t1) = (Node v ls rs)) /\ 
+    ((get_tree_val (snd t1)) > (snd (fst t3))).
+
+Definition tree_up_fail:
+  tree_state -> tree_state -> Prop:=
+    Rels.test(fun t => 
+      match (fst t) with
+      | nil => True
+      | t2::lt => snd (fst t2) >= (get_tree_val (snd t))
+      end).
+
+Fixpoint iter_n_tree_up (n: nat):
+  tree_state -> tree_state -> Prop:=
+  match n with
+  | O => tree_up_fail
+  | S n0 => tree_up_succeed ∘ (iter_n_tree_up n0)
+  end.
+
+Definition heap_tree_up:
+  tree_state -> tree_state -> Prop:=
+  ⋃ (iter_n_tree_up).
+
+Definition left_son_check_tree (t: tree): Prop:=
+  exists v ls rs, t = (Node v ls rs) /\ ~(ls = Leaf) /\ (get_tree_val ls) > v.
+
+Definition right_son_check_tree (t: tree): Prop:=
+  exists v ls rs, t = (Node v ls rs) /\ ~(rs = Leaf) /\ (get_tree_val rs) > v.
+
+Definition swap_down_left (t1 t2: tree) (t: bool*Z*tree): Prop:=
+  exists v ls rs vl lls lrs, t1 = (Node v ls rs) /\ ls = (Node vl lls lrs) /\
+  t2 = (Node v lls lrs) /\ t = (false, vl, rs).
+
+Definition swap_down_right (t1 t2: tree) (t: bool*Z*tree): Prop:=
+  exists v ls rs vr rls rrs, t1 = (Node v ls rs) /\ rs = (Node vr rls rrs) /\
+  t2 = (Node v rls rrs) /\ t = (true, vr, ls).
+
+Definition tree_down_succeed:
+  tree_state -> tree_state -> Prop:=
+    fun t1 t2 => exists t, (t::(fst t1)) = (fst t2) /\ (
+      ((left_son_check_tree (snd t1)) /\ ~(right_son_check_tree (snd t1)) /\ (swap_down_left (snd t1) (snd t2) t)) \/
+      (~(left_son_check_tree (snd t1)) /\ (right_son_check_tree (snd t1)) /\ (swap_down_right (snd t1) (snd t2) t)) \/
+      ((left_son_check_tree (snd t1)) /\ (right_son_check_tree (snd t1)) /\ (exists v ls rs, (snd t1) = (Node v ls rs) /\ (
+        ((get_tree_val rs) > (get_tree_val ls) /\ (swap_down_right (snd t1) (snd t2) t)) \/
+        ((get_tree_val rs) <= (get_tree_val ls) /\ (swap_down_left (snd t1) (snd t2) t)))
+      ))
+    ).
+
+Definition tree_down_fail:
+  tree_state -> tree_state -> Prop:=
+  Rels.test(
+    fun t => (legal_tree_state t) /\ ~(left_son_check_tree (snd t)) /\ ~(right_son_check_tree (snd t))
+  ).
+
+Fixpoint iter_n_tree_down (n: nat):
+  tree_state -> tree_state -> Prop:=
+  match n with
+  | O => tree_down_fail
+  | S n0 => tree_down_succeed ∘ (iter_n_tree_down n0)
+  end.
+
+Definition heap_tree_down:
+  tree_state -> tree_state -> Prop:=
+  ⋃ (iter_n_tree_down).
+
+Ltac try_unfold_tree :=
+  unfold swap_down_left; unfold left_son_check_tree; 
+  unfold swap_down_right; unfold right_son_check_tree;
+  unfold get_tree_val; unfold legal_tree_state; simpl.
+
+Example list1: list Z:= [4;8;5].
+Example tree_state_end: tree_state:=
+  (nil, Node 8 (Node 4 Leaf Leaf) (Node 5 Leaf Leaf)).
+Example tree_state_begin: tree_state:=
+  ([(false,4,(Node 5 Leaf Leaf))]%list, Node 8 Leaf Leaf).
+
+Example test_heap_tree_up:
+  heap_tree_up tree_state_begin tree_state_end.
+Proof.
+  unfold heap_tree_up.
+  unfold_RELS_tac.
+  exists 1%nat. unfold iter_n_tree_up.
+  unfold_RELS_tac.
+  exists tree_state_end.
+  split.
+  + unfold tree_up_succeed.
+    exists (false,4,(Node 5 Leaf Leaf)), nil.
+    unfold tree_state_begin; unfold tree_state_end; simpl.
+    split; [tauto|].
+    split; [tauto|].
+    split.
+    - unfold swap_up_and_combine; simpl.
+      exists 8, Leaf, Leaf; tauto.
+    - lia.
+  + unfold tree_up_fail.
+    unfold_RELS_tac; simpl.
+    tauto.
+Qed.
+
+Example up_fail_val_err: tree_up_fail
+  ([(false,9,(Node 5 Leaf Leaf))]%list, Node 8 Leaf Leaf)
+  ([(false,9,(Node 5 Leaf Leaf))]%list, Node 8 Leaf Leaf).
+Proof.
+  unfold tree_up_fail.
+  unfold_RELS_tac; simpl.
+  split; [lia|tauto].
+Qed.
+
+Example tree_state_begin2: tree_state:=
+  (nil, Node 4 (Node 8 Leaf Leaf) (Node 5 Leaf Leaf)).
+Example tree_state_end2: tree_state:=
+  ([(false,8,(Node 5 Leaf Leaf))]%list, Node 4 Leaf Leaf).
+
+Example test_heap_tree_down:
+  heap_tree_down tree_state_begin2 tree_state_end2.
+Proof.
+  unfold heap_tree_down.
+  unfold_RELS_tac.
+  exists 1%nat. unfold iter_n_tree_down.
+  unfold_RELS_tac.
+  exists tree_state_end2.
+  split.
+  + unfold tree_down_succeed.
+    exists (false,8,(Node 5 Leaf Leaf)).
+    split; [tauto|].
+    right. right. 
+    try_unfold_tree.
+    split. 
+      exists 4, (Node 8 Leaf Leaf), (Node 5 Leaf Leaf).
+      split; [tauto|].
+      split; [discriminate|lia].
+    split.
+      exists 4, (Node 8 Leaf Leaf), (Node 5 Leaf Leaf).
+      split; [tauto|].
+      split; [discriminate|lia].
+    exists 4, (Node 8 Leaf Leaf), (Node 5 Leaf Leaf).
+    split; [tauto|].
+    right.
+    split; [lia|].
+    exists 4, (Node 8 Leaf Leaf), (Node 5 Leaf Leaf), 8, Leaf, Leaf.
+    tauto.
+  + unfold tree_down_fail.
+    unfold_RELS_tac.
+    try_unfold_tree.
+    split; [|tauto].
+    split; [exists 4, Leaf, Leaf; tauto|].
+    split;
+    apply all_not_not_ex; intros;
+    apply all_not_not_ex; intros;
+    apply all_not_not_ex; intros;
+    apply Classical_Prop.or_not_and;
+    apply Classical_Prop.imply_to_or;
+    intros;
+    injection H;
+    intros; subst;
+    apply Classical_Prop.or_not_and;
+    left; tauto.
+Qed.
+
+Example down_fail_val_err: tree_down_fail
+  (nil, Node 9 (Node 8 Leaf Leaf) (Node 5 Leaf Leaf))
+  (nil, Node 9 (Node 8 Leaf Leaf) (Node 5 Leaf Leaf)).
+Proof.
+  unfold tree_down_fail.
+  unfold_RELS_tac; simpl.
+  try_unfold_tree.
+  split; [|tauto].
+  split.
+  + exists 9, (Node 8 Leaf Leaf), (Node 5 Leaf Leaf); tauto.
+  + split;
+    apply all_not_not_ex; intros;
+    apply all_not_not_ex; intros;
+    apply all_not_not_ex; intros;
+    apply Classical_Prop.or_not_and;
+    apply Classical_Prop.imply_to_or;
+    intros;
+    injection H;
+    intros; subst;
+    apply Classical_Prop.or_not_and;
+    right; lia.
+Qed.
